

A Useful Complex-Valued Logic

Michael D. Karayani
mkarajani@gmail.com

October 18, 2025

Abstract

A *useful complex-valued logic* based on three-valued logic (with balanced ternary representation) and assumption that the logical equivalence corresponds to the hypercomplex multiplication operation.

1 Balanced Ternary Algebra

1.1 Definitions

$$1.1.1 \quad \mathbb{N} := \{1, 2, 3, \dots\}$$

$$1.1.2 \quad \mathbb{Z}_3 := \{-1, 0, 1\}$$

$$1.1.3 \quad \forall x, y \in \mathbb{Z}_3:$$

$$1.1.3.1 \quad x \oplus y := (x + y + 4) \bmod 3 - 1$$

$$1.1.3.2 \quad x \otimes y := xy$$

$$1.1.4 \quad \forall x \in \mathbb{Z}_3:$$

$$1.1.4.1 \quad \ominus x := -1 \otimes x$$

$$1.1.4.2 \quad x^{\otimes 0} := 1$$

$$1.1.4.3 \quad \forall n \in \mathbb{N}: x^{\otimes n} := x \otimes x^{\otimes(n-1)}$$

1.2 Corollaries

$$\forall x \in \mathbb{Z}_3:$$

$$1.2.1 \quad x \oplus x = \ominus x \text{ (1.1.3.1, 1.1.4.1)}$$

$$1.2.2 \quad \forall n \in \mathbb{N}:$$

$$1.2.2.1 \quad x^{\otimes(2n-1)} = x \text{ (1.1.4.2, 1.1.4.3)}$$

$$1.2.2.2 \quad x^{\otimes(2n)} = x^{\otimes 2} \text{ (1.1.4.2, 1.1.4.3)}$$

2 Three-Valued Logic

2.1 Definitions

$$2.1.1 \quad \forall x \in \mathbb{Z}_3: \neg x := \ominus x$$

$$2.1.2 \quad \forall x, y \in \mathbb{Z}_3:$$

$$2.1.2.1 \quad x \wedge y := \min(x, y)$$

$$2.1.2.2 \quad x \vee y := \neg(\neg x \wedge \neg y)$$

$$2.1.2.3 \quad x \Rightarrow y := \neg x \vee y$$

$$2.1.2.4 \quad x \Leftrightarrow y := (x \Rightarrow y) \wedge (y \Rightarrow x)$$

2.2 Corollaries

$\forall x, y \in \mathbb{Z}_3$:

$$2.2.1 \quad x \vee y = \max(x, y) \quad (2.1.2.2)$$

$$2.2.2 \quad x \Leftrightarrow y = (x \vee \neg y) \wedge (\neg x \vee y) \quad (2.1.2.3, 2.1.2.4)$$

$$2.2.3 \quad x \Leftrightarrow y = (x \wedge y) \vee (\neg x \wedge \neg y) \quad (2.2.2)$$

2.3 Algebraic Normal Forms

2.3.1 Algorithm

2.3.1.1 Given:

2.3.1.1.1 D : k -vector of sorted values of algebra's domain.

2.3.1.1.2 T : k^2 -vector of the truth table's values for binary operation \circ , where:

$$t_i = d_{\lceil \frac{i}{k} \rceil} \circ d_{(i \bmod k)}$$

2.3.1.2 Find:

2.3.1.2.1 A : k^2 -vector of coefficients for algebraic normal form of binary operation \circ , where:

$$x \circ y = \bigoplus_{i=1}^{k^2} \left(a_i \otimes x^{\otimes \lfloor \frac{i-1}{k} \rfloor} \otimes y^{\otimes ((i-1) \bmod k)} \right)$$

2.3.1.3 Solution:

2.3.1.3.1 $V_{i,j} = d_i^{\otimes(j-1)}$ (Vandermonde matrix of size $k \times k$)

2.3.1.3.2 $P_1 = V^{-1}$ (matrix inversion)

2.3.1.3.3 $P_2 = P_1 \otimes P_1$ (Kronecker product)

2.3.1.3.4 $A = P_2 T$ (matrix multiplication)

2.3.2 Result

$$2.3.2.1 \quad D = \begin{pmatrix} \ominus 1 \\ 0 \\ 1 \end{pmatrix} \quad (2.3.1.1.1)$$

2.3.2.2 $\forall x, y \in \mathbb{Z}_3$:

$$2.3.2.2.1 \quad x \wedge y = \ominus y \oplus y^{\otimes 2} \ominus x \ominus x \otimes y \oplus x^{\otimes 2} \ominus x^{\otimes 2} \otimes y^{\otimes 2} \quad (2.1.2.1, 2.3.1.3.4)$$

$$2.3.2.2.2 \quad x \vee y = \ominus y \ominus y^{\otimes 2} \ominus x \oplus x \otimes y \ominus x^{\otimes 2} \oplus x^{\otimes 2} \otimes y^{\otimes 2} \quad (2.2.1, 2.3.1.3.4)$$

$$2.3.2.2.3 \quad x \Rightarrow y = \ominus y \ominus y^{\otimes 2} \oplus x \ominus x \otimes y \ominus x^{\otimes 2} \oplus x^{\otimes 2} \otimes y^{\otimes 2} \quad (2.1.2.3, 2.3.1.3.4)$$

$$2.3.2.2.4 \quad x \Leftrightarrow y = x \otimes y \quad (2.1.2.4, 2.3.1.3.4)$$

3 Balanced Hypercomplex Algebras

3.1 Definitions

$$3.1.1 \quad \mathbb{C}_3 := \{a \oplus b \otimes i \mid a, b \in \mathbb{Z}_3, i^{\otimes 2} = -1\}$$

$$3.1.2 \quad \mathbb{D}_3 := \{a \oplus b \otimes \varepsilon \mid a, b \in \mathbb{Z}_3, \varepsilon^{\otimes 2} = 0 \wedge \varepsilon \neq 0\}$$

$$3.1.3 \quad \mathbb{S}_3 := \{a \oplus b \otimes j \mid a, b \in \mathbb{Z}_3, j^{\otimes 2} = 1 \wedge j \notin \{-1, 1\}\}$$

3.1.4 $\forall u \in \{i, \varepsilon, j\}, \forall a, b, c, d \in \mathbb{Z}_3: \forall x = a \oplus b \otimes u, \forall y = c \oplus d \otimes u:$

3.1.4.1 $x \oplus y := a \oplus c \oplus (b \oplus d) \otimes u$

3.1.4.2 $x \otimes y := a \otimes c \oplus u^{\otimes 2} \otimes b \otimes d \oplus (a \otimes d \oplus b \otimes c) \otimes u$

3.1.5 $\forall \mathbb{K} \in \{\mathbb{C}_3, \mathbb{D}_3, \mathbb{S}_3\}: \forall x \in \mathbb{K}:$

3.1.5.1 $\ominus x := -1 \otimes x$

3.1.5.2 $x^{\otimes 0} := 1$

3.1.5.3 $\forall n \in \mathbb{N}: x^{\otimes n} := x \otimes x^{\otimes(n-1)}$

3.2 Corollaries

$\forall \mathbb{K} \in \{\mathbb{C}_3, \mathbb{D}_3, \mathbb{S}_3\}: \forall x \in \mathbb{K}:$

3.2.1 $x \oplus x = \ominus x$ (3.1.4.1, 3.1.5.1)

3.2.2 $\forall n \in \mathbb{N}:$

3.2.2.1 $x^{\otimes(4n-3)} = x$ (3.1.5.2, 3.1.5.3)

3.2.2.2 $x^{\otimes(4n-2)} = x^{\otimes 2}$ (3.1.5.2, 3.1.5.3)

3.2.2.3 $x^{\otimes(4n-1)} = x^{\otimes 3}$ (3.1.5.2, 3.1.5.3)

3.2.2.4 $x^{\otimes(4n)} = x^{\otimes 4}$ (3.1.5.2, 3.1.5.3)

3.3 Multiplication Tables (3.1.4.2)

\mathbb{C}_3	$\ominus 1 \ominus i$	$\ominus 1$	$\ominus 1 \oplus i$	$\ominus i$	0	i	$1 \ominus i$	1	$1 \oplus i$
$\ominus 1 \ominus i$	$\ominus i$	$1 \oplus i$	$\ominus 1$	$\ominus 1 \oplus i$	0	$1 \ominus i$	1	$\ominus 1 \ominus i$	i
$\ominus 1$	$1 \oplus i$	1	$1 \ominus i$	i	0	$\ominus i$	$\ominus 1 \oplus i$	$\ominus 1$	$\ominus 1 \ominus i$
$\ominus 1 \oplus i$	$\ominus 1$	$1 \ominus i$	i	$1 \oplus i$	0	$\ominus 1 \ominus i$	$\ominus i$	$\ominus 1 \oplus i$	1
$\ominus i$	$\ominus 1 \oplus i$	i	$1 \oplus i$	$\ominus 1$	0	1	$\ominus 1 \ominus i$	$\ominus i$	$1 \ominus i$
0	0	0	0	0	0	0	0	0	0
i	$1 \ominus i$	$\ominus i$	$\ominus 1 \ominus i$	1	0	$\ominus 1$	$1 \oplus i$	i	$\ominus 1 \oplus i$
$1 \ominus i$	1	$\ominus 1 \oplus i$	$\ominus i$	$\ominus 1 \ominus i$	0	$1 \oplus i$	i	$1 \ominus i$	$\ominus 1$
1	$\ominus 1 \ominus i$	$\ominus 1$	$\ominus 1 \oplus i$	$\ominus i$	0	i	$1 \ominus i$	1	$1 \oplus i$
$1 \oplus i$	i	$\ominus 1 \ominus i$	1	$1 \ominus i$	0	$\ominus 1 \oplus i$	$\ominus 1$	$1 \oplus i$	$\ominus i$

\mathbb{D}_3	$\ominus 1 \ominus \varepsilon$	$\ominus 1$	$\ominus 1 \oplus \varepsilon$	$\ominus \varepsilon$	0	ε	$1 \ominus \varepsilon$	1	$1 \oplus \varepsilon$
$\ominus 1 \ominus \varepsilon$	$1 \ominus \varepsilon$	$1 \oplus \varepsilon$	1	ε	0	$\ominus \varepsilon$	$\ominus 1$	$\ominus 1 \ominus \varepsilon$	$\ominus 1 \oplus \varepsilon$
$\ominus 1$	$1 \oplus \varepsilon$	1	$1 \ominus \varepsilon$	ε	0	$\ominus \varepsilon$	$\ominus 1 \oplus \varepsilon$	$\ominus 1$	$\ominus 1 \ominus \varepsilon$
$\ominus 1 \oplus \varepsilon$	1	$1 \ominus \varepsilon$	$1 \oplus \varepsilon$	ε	0	$\ominus \varepsilon$	$\ominus 1 \ominus \varepsilon$	$\ominus 1 \oplus \varepsilon$	$\ominus 1$
$\ominus \varepsilon$	ε	ε	ε	0	0	0	$\ominus \varepsilon$	$\ominus \varepsilon$	$\ominus \varepsilon$
0	0	0	0	0	0	0	0	0	0
ε	$\ominus \varepsilon$	$\ominus \varepsilon$	$\ominus \varepsilon$	0	0	0	ε	ε	ε
$1 \ominus \varepsilon$	$\ominus 1$	$\ominus 1 \oplus \varepsilon$	$\ominus 1 \ominus \varepsilon$	$\ominus \varepsilon$	0	ε	$1 \oplus \varepsilon$	$1 \ominus \varepsilon$	1
1	$\ominus 1 \ominus \varepsilon$	$\ominus 1$	$\ominus 1 \oplus \varepsilon$	$\ominus \varepsilon$	0	ε	$1 \ominus \varepsilon$	1	$1 \oplus \varepsilon$
$1 \oplus \varepsilon$	$\ominus 1 \oplus \varepsilon$	$\ominus 1 \ominus \varepsilon$	$\ominus 1$	$\ominus \varepsilon$	0	ε	1	$1 \oplus \varepsilon$	$1 \ominus \varepsilon$

\mathbb{S}_3	$\ominus 1 \ominus j$	$\ominus 1$	$\ominus 1 \oplus j$	$\ominus j$	0	j	$1 \ominus j$	1	$1 \oplus j$
$\ominus 1 \ominus j$	$\ominus 1 \ominus j$	$1 \oplus j$	0	$1 \oplus j$	0	$\ominus 1 \ominus j$	0	$\ominus 1 \ominus j$	$1 \oplus j$
$\ominus 1$	$1 \oplus j$	1	$1 \ominus j$	j	0	$\ominus j$	$\ominus 1 \oplus j$	$\ominus 1$	$\ominus 1 \ominus j$
$\ominus 1 \oplus j$	0	$1 \ominus j$	$\ominus 1 \oplus j$	$\ominus 1 \oplus j$	0	$1 \ominus j$	$1 \ominus j$	$\ominus 1 \oplus j$	0
$\ominus j$	$1 \oplus j$	j	$\ominus 1 \oplus j$	1	0	$\ominus 1$	$1 \ominus j$	$\ominus j$	$\ominus 1 \ominus j$
0	0	0	0	0	0	0	0	0	0
j	$\ominus 1 \ominus j$	$\ominus j$	$1 \ominus j$	$\ominus 1$	0	1	$\ominus 1 \oplus j$	j	$1 \oplus j$
$1 \ominus j$	0	$\ominus 1 \oplus j$	$1 \ominus j$	$1 \ominus j$	0	$\ominus 1 \oplus j$	$\ominus 1 \oplus j$	$1 \ominus j$	0
1	$\ominus 1 \ominus j$	$\ominus 1$	$\ominus 1 \oplus j$	$\ominus j$	0	j	$1 \ominus j$	1	$1 \oplus j$
$1 \oplus j$	$1 \oplus j$	$\ominus 1 \ominus j$	0	$\ominus 1 \ominus j$	0	$1 \oplus j$	0	$1 \oplus j$	$\ominus 1 \ominus j$

4 Hypercomplex-Valued Logics

4.1 Definitions

$\forall \mathbb{K} \in \{\mathbb{C}_3, \mathbb{D}_3, \mathbb{S}_3\}$:

4.1.1 $\forall x \in \mathbb{K}$:

$$4.1.1.1 \neg x := \ominus x$$

$$4.1.1.2 x \wedge \ominus 1 := \ominus 1$$

$$4.1.1.3 x \wedge 1 := x$$

4.1.2 $\forall x, y \in \mathbb{K}$:

$$4.1.2.1 x \vee y := \neg(\neg x \wedge \neg y)$$

$$4.1.2.2 x \Rightarrow y := \neg x \vee y$$

$$4.1.2.3 x \Leftrightarrow y := (x \Rightarrow y) \wedge (y \Rightarrow x)$$

4.2 Assumptions

$\forall \mathbb{K} \in \{\mathbb{C}_3, \mathbb{D}_3, \mathbb{S}_3\}$:

$$4.2.1 \forall x, y \in \mathbb{K}: x \Leftrightarrow y = x \otimes y$$

$$4.2.2 \forall x, y, z \in \mathbb{K}: (x \wedge y) \wedge z = x \wedge (y \wedge z)$$

$$4.2.3 \forall x, y \in \mathbb{K} \setminus \{0\}: x \wedge y \neq 0$$

4.3 Corollaries

$\forall \mathbb{K} \in \{\mathbb{C}_3, \mathbb{D}_3, \mathbb{S}_3\}$:

4.3.1 $\forall x \in \mathbb{K}$:

$$4.3.1.1 x \vee \ominus 1 = x \text{ (4.1.1.3, 4.1.2.1)}$$

$$4.3.1.2 x \vee 1 = 1 \text{ (4.1.1.2, 4.1.2.1)}$$

4.3.2 $\forall x, y \in \mathbb{K}$:

$$4.3.2.1 x \Leftrightarrow y = (x \vee \neg y) \wedge (\neg x \vee y) \text{ (4.1.2.2, 4.1.2.3)}$$

$$4.3.2.2 x \Leftrightarrow y = (x \wedge y) \vee (\neg x \wedge \neg y) \text{ (4.3.2.1)}$$

$$4.3.2.3 x \otimes y = (x \vee \neg y) \wedge (\neg x \vee y) \text{ (4.2.1, 4.3.2.1)}$$

$$4.3.3 \forall x, y, z \in \mathbb{K}: (x \vee y) \vee z = x \vee (y \vee z) \text{ (4.1.2.1, 4.2.2)}$$

$$4.3.4 \forall x, y \in \mathbb{K} \setminus \{0\}: x \vee y \neq 0 \text{ (4.1.2.1, 4.2.3)}$$

4.4 Conjunction Values Problem

4.4.1 Values by Definitions (2.1.2.1, 4.1.1.2, 4.1.1.3)

\wedge	$\ominus 1 \ominus u$	$\ominus 1$	$\ominus 1 \oplus u$	$\ominus u$	0	u	$1 \ominus u$	1	$1 \oplus u$
$\ominus 1 \ominus u$	x_1	$\ominus 1$	x_2	x_3	x_4	x_5	x_6	$\ominus 1 \ominus u$	x_7
$\ominus 1$	$\ominus 1$	$\ominus 1$	$\ominus 1$	$\ominus 1$	$\ominus 1$	$\ominus 1$	$\ominus 1$	$\ominus 1$	$\ominus 1$
$\ominus 1 \oplus u$	x_2	$\ominus 1$	x_8	x_9	x_{10}	x_{11}	x_{12}	$\ominus 1 \oplus u$	x_{13}
$\ominus u$	x_3	$\ominus 1$	x_9	x_{14}	x_{15}	x_{16}	x_{17}	$\ominus u$	x_{18}
0	x_4	$\ominus 1$	x_{10}	x_{15}	0	x_{19}	x_{20}	0	x_{21}
u	x_5	$\ominus 1$	x_{11}	x_{16}	x_{19}	x_{22}	x_{23}	u	x_{24}
$1 \ominus u$	x_6	$\ominus 1$	x_{12}	x_{17}	x_{20}	x_{23}	x_{25}	$1 \ominus u$	x_{26}
1	$\ominus 1 \ominus u$	$\ominus 1$	$\ominus 1 \oplus u$	$\ominus u$	0	u	$1 \ominus u$	1	$1 \oplus u$
$1 \oplus u$	x_7	$\ominus 1$	x_{13}	x_{18}	x_{21}	x_{24}	x_{26}	$1 \oplus u$	x_{27}

4.4.2 Searching Values by Assumptions

$\forall \mathbb{K} \in \{\mathbb{C}_3, \mathbb{D}_3, \mathbb{S}_3\} :$

4.4.2.1 $\mathcal{B}(\mathbb{K}) = \{X \in \mathbb{K}^{27} \mid X \text{ satisfies basic assumptions (4.2.1, 4.2.2)}\}^1$

4.4.2.2 $\mathcal{C}(\mathbb{K}) = \{Y \in \mathcal{B}(\mathbb{K}) \mid Y \text{ satisfies crisp connectives assumption (4.2.3)}\}^2$

4.4.3 Search Results

4.4.3.1 By basic assumptions (4.4.2.1):

4.4.3.1.1 $|\mathcal{B}(\mathbb{C}_3)| = 2$ (see on [github.io](https://github.com))

4.4.3.1.2 $|\mathcal{B}(\mathbb{D}_3)| = 1\,492$ (see on [github.io](https://github.com))

4.4.3.1.3 $|\mathcal{B}(\mathbb{S}_3)| = 15$ (see on [github.io](https://github.com))

4.4.3.2 By crisp connectives assumption (4.4.2.2):

$$4.4.3.2.1 \mathcal{C}(\mathbb{C}_3) = \left\{ \left(\begin{array}{c} \ominus 1 \oplus i \\ i \\ 1 \oplus i \\ 0 \\ \ominus i \\ 1 \\ 1 \ominus i \\ \ominus i \\ 1 \ominus i \\ 0 \\ 1 \oplus i \\ \ominus 1 \ominus i \\ 1 \\ \ominus 1 \ominus i \\ 0 \\ 1 \\ i \\ \ominus 1 \oplus i \\ 0 \\ 0 \\ 0 \\ 1 \ominus i \\ \ominus 1 \oplus i \\ \ominus 1 \ominus i \\ 1 \oplus i \\ \ominus i \\ \ominus i \\ i \end{array} \right), \left(\begin{array}{c} i \\ \ominus i \\ 1 \ominus i \\ 0 \\ 1 \oplus i \\ \ominus 1 \oplus i \\ \ominus 1 \ominus i \\ i \\ 0 \\ 1 \ominus i \\ 1 \oplus i \\ 1 \\ 1 \oplus i \\ \ominus 1 \oplus i \\ \ominus 1 \ominus i \\ i \\ 1 \ominus i \\ \ominus 1 \oplus i \\ 0 \\ 0 \\ 0 \\ \ominus 1 \oplus i \\ \ominus 1 \ominus i \\ \ominus i \\ \ominus i \\ i \\ 1 \ominus i \end{array} \right) \right\}$$

4.4.3.2.2 $\mathcal{C}(\mathbb{D}_3) = \emptyset$

4.4.3.2.3 $\mathcal{C}(\mathbb{S}_3) = \emptyset$

¹ $\forall \mathbb{K} \in \{\mathbb{C}_3, \mathbb{D}_3, \mathbb{S}_3\}$ there are $3 \times |\mathbb{K}^{27}| = 3 \times 9^{27} \approx 1,7445 \times 10^{26}$ variants to check.

²These are candidates for a *useful hypercomplex-valued logic*: their logical connectives are closed on a set of the crisp values $(\mathbb{K} \setminus \{0\})$.

5 Two Candidates

5.1 Truth Tables (4.1.2.1, 4.1.2.2, 4.1.2.3, 4.4.1, 4.4.3.2.1)

5.1.1 First candidate

\wedge	$\ominus 1 \ominus i$	$\ominus 1$	$\ominus 1 \oplus i$	$\ominus i$	0	i	$1 \ominus i$	1	$1 \oplus i$
$\ominus 1 \ominus i$	$\ominus 1 \oplus i$	$\ominus 1$	i	$1 \oplus i$	0	$\ominus i$	1	$\ominus 1 \ominus i$	$1 \ominus i$
$\ominus 1$	$\ominus 1$	$\ominus 1$	$\ominus 1$	$\ominus 1$	$\ominus 1$	$\ominus 1$	$\ominus 1$	$\ominus 1$	$\ominus 1$
$\ominus 1 \oplus i$	i	$\ominus 1$	$\ominus i$	$1 \ominus i$	0	$1 \oplus i$	$\ominus 1 \ominus i$	$\ominus 1 \oplus i$	1
$\ominus i$	$1 \oplus i$	$\ominus 1$	$1 \ominus i$	$\ominus 1 \ominus i$	0	1	i	$\ominus i$	$\ominus 1 \oplus i$
0	0	$\ominus 1$	0	0	0	0	0	0	0
i	$\ominus i$	$\ominus 1$	$1 \oplus i$	1	0	$1 \ominus i$	$\ominus 1 \oplus i$	i	$\ominus 1 \ominus i$
$1 \ominus i$	1	$\ominus 1$	$\ominus 1 \ominus i$	i	0	$\ominus 1 \oplus i$	$1 \oplus i$	$1 \ominus i$	$\ominus i$
1	$\ominus 1 \ominus i$	$\ominus 1$	$\ominus 1 \oplus i$	$\ominus i$	0	i	$1 \ominus i$	1	$1 \oplus i$
$1 \oplus i$	$1 \ominus i$	$\ominus 1$	1	$\ominus 1 \oplus i$	0	$\ominus 1 \ominus i$	$\ominus i$	$1 \oplus i$	i

\vee	$\ominus 1 \ominus i$	$\ominus 1$	$\ominus 1 \oplus i$	$\ominus i$	0	i	$1 \ominus i$	1	$1 \oplus i$
$\ominus 1 \ominus i$	$\ominus i$	$\ominus 1 \ominus i$	i	$1 \oplus i$	0	$1 \ominus i$	$\ominus 1$	1	$\ominus 1 \oplus i$
$\ominus 1$	$\ominus 1 \ominus i$	$\ominus 1$	$\ominus 1 \oplus i$	$\ominus i$	0	i	$1 \ominus i$	1	$1 \oplus i$
$\ominus 1 \oplus i$	i	$\ominus 1 \oplus i$	$\ominus 1 \ominus i$	$1 \ominus i$	0	$\ominus i$	$1 \oplus i$	1	$\ominus 1$
$\ominus i$	$1 \oplus i$	$\ominus i$	$1 \ominus i$	$\ominus 1 \oplus i$	0	$\ominus 1$	$\ominus 1 \ominus i$	1	i
0	0	0	0	0	0	0	0	1	0
i	$1 \ominus i$	i	$\ominus i$	$\ominus 1$	0	$1 \oplus i$	$\ominus 1 \oplus i$	1	$\ominus 1 \ominus i$
$1 \ominus i$	$\ominus 1$	$1 \ominus i$	$1 \oplus i$	$\ominus 1 \ominus i$	0	$\ominus 1 \oplus i$	i	1	$\ominus i$
1	1	1	1	1	1	1	1	1	1
$1 \oplus i$	$\ominus 1 \oplus i$	$1 \oplus i$	$\ominus 1$	i	0	$\ominus 1 \ominus i$	$\ominus i$	1	$1 \ominus i$

\Rightarrow	$\ominus 1 \ominus i$	$\ominus 1$	$\ominus 1 \oplus i$	$\ominus i$	0	i	$1 \ominus i$	1	$1 \oplus i$
$\ominus 1 \ominus i$	$\ominus 1 \oplus i$	$1 \oplus i$	$\ominus 1$	i	0	$\ominus 1 \ominus i$	$\ominus i$	1	$1 \ominus i$
$\ominus 1$	1	1	1	1	1	1	1	1	1
$\ominus 1 \oplus i$	$\ominus 1$	$1 \ominus i$	$1 \oplus i$	$\ominus 1 \ominus i$	0	$\ominus 1 \oplus i$	i	1	$\ominus i$
$\ominus i$	$1 \ominus i$	i	$\ominus i$	$\ominus 1$	0	$1 \oplus i$	$\ominus 1 \oplus i$	1	$\ominus 1 \ominus i$
0	0	0	0	0	0	0	0	1	0
i	$1 \oplus i$	$\ominus i$	$1 \ominus i$	$\ominus 1 \oplus i$	0	$\ominus 1$	$\ominus 1 \ominus i$	1	i
$1 \ominus i$	i	$\ominus 1 \oplus i$	$\ominus 1 \ominus i$	$1 \ominus i$	0	$\ominus i$	$1 \oplus i$	1	$\ominus 1$
1	$\ominus 1 \ominus i$	$\ominus 1$	$\ominus 1 \oplus i$	$\ominus i$	0	i	$1 \ominus i$	1	$1 \oplus i$
$1 \oplus i$	$\ominus i$	$\ominus 1 \ominus i$	i	$1 \oplus i$	0	$1 \ominus i$	$\ominus 1$	1	$\ominus 1 \oplus i$

\Leftrightarrow	$\ominus 1 \ominus i$	$\ominus 1$	$\ominus 1 \oplus i$	$\ominus i$	0	i	$1 \ominus i$	1	$1 \oplus i$
$\ominus 1 \ominus i$	$\ominus i$	$1 \oplus i$	$\ominus 1$	$\ominus 1 \oplus i$	0	$1 \ominus i$	1	$\ominus 1 \ominus i$	i
$\ominus 1$	$1 \oplus i$	1	$1 \ominus i$	i	0	$\ominus i$	$\ominus 1 \oplus i$	$\ominus 1$	$\ominus 1 \ominus i$
$\ominus 1 \oplus i$	$\ominus 1$	$1 \ominus i$	i	$1 \oplus i$	0	$\ominus 1 \ominus i$	$\ominus i$	$\ominus 1 \oplus i$	1
$\ominus i$	$\ominus 1 \oplus i$	i	$1 \oplus i$	$\ominus 1$	0	1	$\ominus 1 \ominus i$	$\ominus i$	$1 \ominus i$
0	0	0	0	0	0	0	0	0	0
i	$1 \ominus i$	$\ominus i$	$\ominus 1 \ominus i$	1	0	$\ominus 1$	$1 \oplus i$	i	$\ominus 1 \oplus i$
$1 \ominus i$	1	$\ominus 1 \oplus i$	$\ominus i$	$\ominus 1 \ominus i$	0	$1 \oplus i$	i	$1 \ominus i$	$\ominus 1$
1	$\ominus 1 \ominus i$	$\ominus 1$	$\ominus 1 \oplus i$	$\ominus i$	0	i	$1 \ominus i$	1	$1 \oplus i$
$1 \oplus i$	i	$\ominus 1 \ominus i$	1	$1 \ominus i$	0	$\ominus 1 \oplus i$	$\ominus 1$	$1 \oplus i$	$\ominus i$

5.1.2 Second candidate

\wedge	$\ominus 1 \ominus i$	$\ominus 1$	$\ominus 1 \oplus i$	$\ominus i$	0	i	$1 \ominus i$	1	$1 \oplus i$
$\ominus 1 \ominus i$	i	$\ominus 1$	$\ominus i$	$1 \ominus i$	0	$1 \oplus i$	1	$\ominus 1 \ominus i$	$\ominus 1 \oplus i$
$\ominus 1$	$\ominus 1$	$\ominus 1$	$\ominus 1$	$\ominus 1$	$\ominus 1$	$\ominus 1$	$\ominus 1$	$\ominus 1$	$\ominus 1$
$\ominus 1 \oplus i$	$\ominus i$	$\ominus 1$	$\ominus 1 \ominus i$	i	0	$1 \ominus i$	$1 \oplus i$	$\ominus 1 \oplus i$	1
$\ominus i$	$1 \ominus i$	$\ominus 1$	i	$1 \oplus i$	0	1	$\ominus 1 \oplus i$	$\ominus i$	$\ominus 1 \ominus i$
0	0	$\ominus 1$	0	0	0	0	0	0	0
i	$1 \oplus i$	$\ominus 1$	$1 \ominus i$	1	0	$\ominus 1 \oplus i$	$\ominus 1 \ominus i$	i	$\ominus i$
$1 \ominus i$	1	$\ominus 1$	$1 \oplus i$	$\ominus 1 \oplus i$	0	$\ominus 1 \ominus i$	$\ominus i$	$1 \ominus i$	i
1	$\ominus 1 \ominus i$	$\ominus 1$	$\ominus 1 \oplus i$	$\ominus i$	0	i	$1 \ominus i$	1	$1 \oplus i$
$1 \oplus i$	$\ominus 1 \oplus i$	$\ominus 1$	1	$\ominus 1 \ominus i$	0	$\ominus i$	i	$1 \oplus i$	$1 \ominus i$
\vee	$\ominus 1 \ominus i$	$\ominus 1$	$\ominus 1 \oplus i$	$\ominus i$	0	i	$1 \ominus i$	1	$1 \oplus i$
$\ominus 1 \ominus i$	$\ominus 1 \oplus i$	$\ominus 1 \ominus i$	$\ominus i$	i	0	$1 \oplus i$	$\ominus 1$	1	$1 \ominus i$
$\ominus 1$	$\ominus 1 \ominus i$	$\ominus 1$	$\ominus 1 \oplus i$	$\ominus i$	0	i	$1 \ominus i$	1	$1 \oplus i$
$\ominus 1 \oplus i$	$\ominus i$	$\ominus 1 \oplus i$	i	$1 \oplus i$	0	$1 \ominus i$	$\ominus 1 \ominus i$	1	$\ominus 1$
$\ominus i$	i	$\ominus i$	$1 \oplus i$	$1 \ominus i$	0	$\ominus 1$	$\ominus 1 \oplus i$	1	$\ominus 1 \ominus i$
0	0	0	0	0	0	0	0	1	0
i	$1 \oplus i$	i	$1 \ominus i$	$\ominus 1$	0	$\ominus 1 \ominus i$	$\ominus i$	1	$\ominus 1 \oplus i$
$1 \ominus i$	$\ominus 1$	$1 \ominus i$	$\ominus 1 \ominus i$	$\ominus 1 \oplus i$	0	$\ominus i$	$1 \oplus i$	1	i
1	1	1	1	1	1	1	1	1	1
$1 \oplus i$	$1 \ominus i$	$1 \oplus i$	$\ominus 1$	$\ominus 1 \ominus i$	0	$\ominus 1 \oplus i$	i	1	$\ominus i$
\Rightarrow	$\ominus 1 \ominus i$	$\ominus 1$	$\ominus 1 \oplus i$	$\ominus i$	0	i	$1 \ominus i$	1	$1 \oplus i$
$\ominus 1 \ominus i$	$1 \ominus i$	$1 \oplus i$	$\ominus 1$	$\ominus 1 \ominus i$	0	$\ominus 1 \oplus i$	i	1	$\ominus i$
$\ominus 1$	1	1	1	1	1	1	1	1	1
$\ominus 1 \oplus i$	$\ominus 1$	$1 \ominus i$	$\ominus 1 \ominus i$	$\ominus 1 \oplus i$	0	$\ominus i$	$1 \oplus i$	1	i
$\ominus i$	$1 \oplus i$	i	$1 \ominus i$	$\ominus 1$	0	$\ominus 1 \ominus i$	$\ominus i$	1	$\ominus 1 \oplus i$
0	0	0	0	0	0	0	0	1	0
i	i	$\ominus i$	$1 \oplus i$	$1 \ominus i$	0	$\ominus 1$	$\ominus 1 \oplus i$	1	$\ominus 1 \ominus i$
$1 \ominus i$	$\ominus i$	$\ominus 1 \oplus i$	i	$1 \oplus i$	0	$1 \ominus i$	$\ominus 1 \ominus i$	1	$\ominus 1$
1	$\ominus 1 \ominus i$	$\ominus 1$	$\ominus 1 \oplus i$	$\ominus i$	0	i	$1 \ominus i$	1	$1 \oplus i$
$1 \oplus i$	$\ominus 1 \oplus i$	$\ominus 1 \ominus i$	$\ominus i$	i	0	$1 \oplus i$	$\ominus 1$	1	$1 \ominus i$
\Leftrightarrow	$\ominus 1 \ominus i$	$\ominus 1$	$\ominus 1 \oplus i$	$\ominus i$	0	i	$1 \ominus i$	1	$1 \oplus i$
$\ominus 1 \ominus i$	$\ominus i$	$1 \oplus i$	$\ominus 1$	$\ominus 1 \oplus i$	0	$1 \ominus i$	1	$\ominus 1 \ominus i$	i
$\ominus 1$	$1 \oplus i$	1	$1 \ominus i$	i	0	$\ominus i$	$\ominus 1 \oplus i$	$\ominus 1$	$\ominus 1 \ominus i$
$\ominus 1 \oplus i$	$\ominus 1$	$1 \ominus i$	i	$1 \oplus i$	0	$\ominus 1 \ominus i$	$\ominus i$	$\ominus 1 \oplus i$	1
$\ominus i$	$\ominus 1 \oplus i$	i	$1 \oplus i$	$\ominus 1$	0	1	$\ominus 1 \ominus i$	$\ominus i$	$1 \ominus i$
0	0	0	0	0	0	0	0	0	0
i	$1 \ominus i$	$\ominus i$	$\ominus 1 \ominus i$	1	0	$\ominus 1$	$1 \oplus i$	i	$\ominus 1 \oplus i$
$1 \ominus i$	1	$\ominus 1 \oplus i$	$\ominus i$	$\ominus 1 \ominus i$	0	$1 \oplus i$	i	$1 \ominus i$	$\ominus 1$
1	$\ominus 1 \ominus i$	$\ominus 1$	$\ominus 1 \oplus i$	$\ominus i$	0	i	$1 \ominus i$	1	$1 \oplus i$
$1 \oplus i$	i	$\ominus 1 \ominus i$	1	$1 \ominus i$	0	$\ominus 1 \oplus i$	$\ominus 1$	$1 \oplus i$	$\ominus i$

5.3 Functional Equivalence by Logical Connectives

5.3.1 Common values (5.1.1, 5.1.2)

5.3.1.1 By results:

$$5.3.1.1.1 \quad (\ominus 1 \ominus i) \wedge 0 = 0$$

$$5.3.1.1.2 \quad (\ominus 1 \ominus i) \wedge (1 \ominus i) = 1$$

$$5.3.1.1.3 \quad (\ominus 1 \oplus i) \wedge 0 = 0$$

$$5.3.1.1.4 \quad (\ominus 1 \oplus i) \wedge (1 \oplus i) = 1$$

$$5.3.1.1.5 \quad \ominus i \wedge 0 = 0$$

$$5.3.1.1.6 \quad \ominus i \wedge i = 1$$

$$5.3.1.1.7 \quad 0 \wedge i = 0$$

$$5.3.1.1.8 \quad 0 \wedge (1 \ominus i) = 0$$

$$5.3.1.1.9 \quad 0 \wedge (1 \oplus i) = 0$$

5.3.1.2 By equations:

$$5.3.1.2.1 \quad (\ominus 1 \oplus i) \wedge (1 \ominus i) = \ominus i \wedge \ominus i = (i \wedge i) \wedge (i \wedge i)$$

$$5.3.1.2.2 \quad \ominus i \wedge (1 \oplus i) = i \wedge (1 \ominus i)$$

5.3.2 Generalization

5.3.2.1 Definitions:

$$5.3.2.1.1 \quad \aleph := i \wedge i$$

$$5.3.2.1.2 \quad \beth := \aleph \wedge \aleph$$

5.3.2.2 Corollaries (5.1.1, 5.1.2, 5.3.2.1.1, 5.3.2.1.2):

$$5.3.2.2.1 \quad \begin{pmatrix} \aleph \\ \beth \end{pmatrix} \in \left\{ \begin{pmatrix} 1 \ominus i \\ 1 \oplus i \end{pmatrix}, \begin{pmatrix} \ominus 1 \oplus i \\ \ominus 1 \ominus i \end{pmatrix} \right\}$$

$$5.3.2.2.2 \quad \ominus i \wedge \ominus i = \ominus \beth$$

$$5.3.2.2.3 \quad \ominus i \wedge \ominus \beth = \beth$$

$$5.3.2.2.4 \quad \ominus i \wedge \ominus \aleph = \aleph$$

$$5.3.2.2.5 \quad \ominus i \wedge \aleph = i$$

$$5.3.2.2.6 \quad \ominus i \wedge \beth = \ominus \aleph$$

$$5.3.2.2.7 \quad \ominus \beth \wedge \ominus \beth = \ominus \aleph$$

$$5.3.2.2.8 \quad \ominus \beth \wedge \ominus \aleph = i$$

$$5.3.2.2.9 \quad \ominus \beth \wedge 0 = 0$$

$$5.3.2.2.10 \quad \ominus \beth \wedge \aleph = 1$$

$$5.3.2.2.11 \quad \ominus \beth \wedge \beth = \aleph$$

$$5.3.2.2.12 \quad \ominus \beth \wedge i = \ominus i$$

$$5.3.2.2.13 \quad \ominus \aleph \wedge \ominus \aleph = \ominus i$$

$$5.3.2.2.14 \quad \ominus \aleph \wedge 0 = 0$$

$$5.3.2.2.15 \quad \ominus \aleph \wedge \aleph = \ominus \beth$$

$$5.3.2.2.16 \quad \ominus \aleph \wedge \beth = 1$$

$$5.3.2.2.17 \quad \ominus \aleph \wedge i = \beth$$

$$5.3.2.2.18 \quad 0 \wedge \aleph = 0$$

$$5.3.2.2.19 \quad 0 \wedge \beth = 0$$

$$5.3.2.2.20 \quad \aleph \wedge \beth = \ominus i$$

$$5.3.2.2.21 \quad \aleph \wedge i = \ominus \aleph$$

$$5.3.2.2.22 \quad \beth \wedge \beth = i$$

$$5.3.2.2.23 \quad \beth \wedge i = \ominus \beth$$

6 A Useful Complex-Valued Logic

6.1 Truth Tables (5.1.1, 5.1.2, 5.3.2.1.1, 5.3.2.1.2, 5.3.2.2)

\wedge	$\ominus 1$	$\ominus i$	$\ominus \sqsupset$	$\ominus \aleph$	0	\aleph	\sqsupset	i	1
$\ominus 1$	$\ominus 1$	$\ominus 1$	$\ominus 1$	$\ominus 1$	$\ominus 1$	$\ominus 1$	$\ominus 1$	$\ominus 1$	$\ominus 1$
$\ominus i$	$\ominus 1$	$\ominus \sqsupset$	\sqsupset	\aleph	0	i	$\ominus \aleph$	1	$\ominus i$
$\ominus \sqsupset$	$\ominus 1$	\sqsupset	$\ominus \aleph$	i	0	1	\aleph	$\ominus i$	$\ominus \sqsupset$
$\ominus \aleph$	$\ominus 1$	\aleph	i	$\ominus i$	0	$\ominus \sqsupset$	1	\sqsupset	$\ominus \aleph$
0	$\ominus 1$	0	0	0	0	0	0	0	0
\aleph	$\ominus 1$	i	1	$\ominus \sqsupset$	0	\sqsupset	$\ominus i$	$\ominus \aleph$	\aleph
\sqsupset	$\ominus 1$	$\ominus \aleph$	\aleph	1	0	$\ominus i$	i	$\ominus \sqsupset$	\sqsupset
i	$\ominus 1$	1	$\ominus i$	\sqsupset	0	$\ominus \aleph$	$\ominus \sqsupset$	\aleph	i
1	$\ominus 1$	$\ominus i$	$\ominus \sqsupset$	$\ominus \aleph$	0	\aleph	\sqsupset	i	1

\vee	$\ominus 1$	$\ominus i$	$\ominus \sqsupset$	$\ominus \aleph$	0	\aleph	\sqsupset	i	1
$\ominus 1$	$\ominus 1$	$\ominus i$	$\ominus \sqsupset$	$\ominus \aleph$	0	\aleph	\sqsupset	i	1
$\ominus i$	$\ominus i$	$\ominus \aleph$	\sqsupset	\aleph	0	$\ominus \sqsupset$	i	$\ominus 1$	1
$\ominus \sqsupset$	$\ominus \sqsupset$	\sqsupset	$\ominus i$	i	0	$\ominus 1$	$\ominus \aleph$	\aleph	1
$\ominus \aleph$	$\ominus \aleph$	\aleph	i	$\ominus \sqsupset$	0	\sqsupset	$\ominus 1$	$\ominus i$	1
0	0	0	0	0	0	0	0	0	1
\aleph	\aleph	$\ominus \sqsupset$	$\ominus 1$	\sqsupset	0	i	$\ominus i$	$\ominus \aleph$	1
\sqsupset	\sqsupset	i	$\ominus \aleph$	$\ominus 1$	0	$\ominus i$	\aleph	$\ominus \sqsupset$	1
i	i	$\ominus 1$	\aleph	$\ominus i$	0	$\ominus \aleph$	$\ominus \sqsupset$	\sqsupset	1
1	1	1	1	1	1	1	1	1	1

\Rightarrow	$\ominus 1$	$\ominus i$	$\ominus \sqsupset$	$\ominus \aleph$	0	\aleph	\sqsupset	i	1
$\ominus 1$	1	1	1	1	1	1	1	1	1
$\ominus i$	i	$\ominus 1$	\aleph	$\ominus i$	0	$\ominus \aleph$	$\ominus \sqsupset$	\sqsupset	1
$\ominus \sqsupset$	\sqsupset	i	$\ominus \aleph$	$\ominus 1$	0	$\ominus i$	\aleph	$\ominus \sqsupset$	1
$\ominus \aleph$	\aleph	$\ominus \sqsupset$	$\ominus 1$	\sqsupset	0	i	$\ominus i$	$\ominus \aleph$	1
0	0	0	0	0	0	0	0	0	1
\aleph	$\ominus \aleph$	\aleph	i	$\ominus \sqsupset$	0	\sqsupset	$\ominus 1$	$\ominus i$	1
\sqsupset	$\ominus \sqsupset$	\sqsupset	$\ominus i$	i	0	$\ominus 1$	$\ominus \aleph$	\aleph	1
i	$\ominus i$	$\ominus \aleph$	\sqsupset	\aleph	0	$\ominus \sqsupset$	i	$\ominus 1$	1
1	$\ominus 1$	$\ominus i$	$\ominus \sqsupset$	$\ominus \aleph$	0	\aleph	\sqsupset	i	1

\Leftrightarrow	$\ominus 1$	$\ominus i$	$\ominus \sqsupset$	$\ominus \aleph$	0	\aleph	\sqsupset	i	1
$\ominus 1$	1	i	\sqsupset	\aleph	0	$\ominus \aleph$	$\ominus \sqsupset$	$\ominus i$	$\ominus 1$
$\ominus i$	i	$\ominus 1$	$\ominus \aleph$	\sqsupset	0	$\ominus \sqsupset$	\aleph	1	$\ominus i$
$\ominus \sqsupset$	\sqsupset	$\ominus \aleph$	$\ominus i$	$\ominus 1$	0	1	i	\aleph	$\ominus \sqsupset$
$\ominus \aleph$	\aleph	\sqsupset	$\ominus 1$	i	0	$\ominus i$	1	$\ominus \sqsupset$	$\ominus \aleph$
0	0	0	0	0	0	0	0	0	0
\aleph	$\ominus \aleph$	$\ominus \sqsupset$	1	$\ominus i$	0	i	$\ominus 1$	\sqsupset	\aleph
\sqsupset	$\ominus \sqsupset$	\aleph	i	1	0	$\ominus 1$	$\ominus i$	$\ominus \aleph$	\sqsupset
i	$\ominus i$	1	\aleph	$\ominus \sqsupset$	0	\sqsupset	$\ominus \aleph$	$\ominus 1$	i
1	$\ominus 1$	$\ominus i$	$\ominus \sqsupset$	$\ominus \aleph$	0	\aleph	\sqsupset	i	1

6.2 Application

The values i and $\ominus i$ can be used as truth values of cross-world predicates in coherent worlds.